thys/Lambda_Free_RPOs/Lambda_Free_RPOs.thy
@@ -20,8 +20,8 @@ definition arity_sym :: "nat \<Rightarrow> enat" where
 definition arity_var :: "nat \<Rightarrow> enat" where
   "arity_var n = \<infinity>"
 
-definition ground_head_vars :: "nat \<Rightarrow> nat set" where
-  "ground_head_vars x = UNIV"
+definition ground_head_var :: "nat \<Rightarrow> nat set" where
+  "ground_head_var x = UNIV"
 
 definition gt_sym :: "nat \<Rightarrow> nat \<Rightarrow> bool" where
   "gt_sym g f \<longleftrightarrow> g > f"
@@ -29,10 +29,10 @@ definition gt_sym :: "nat \<Rightarrow> nat \<Rightarrow> bool" where
 sublocale app: rpo_app gt_sym len_lexext
   by unfold_locales (auto simp: gt_sym_def intro: wf_less[folded wfP_def])
 
-sublocale std: rpo ground_head_vars gt_sym "\<lambda>f. len_lexext" arity_sym arity_var
-  by unfold_locales (auto simp: arity_var_def arity_sym_def ground_head_vars_def)
+sublocale std: rpo ground_head_var gt_sym "\<lambda>f. len_lexext" arity_sym arity_var
+  by unfold_locales (auto simp: arity_var_def arity_sym_def ground_head_var_def)
 
-sublocale optim: rpo_optim ground_head_vars gt_sym "\<lambda>f. len_lexext" arity_sym arity_var
+sublocale optim: rpo_optim ground_head_var gt_sym "\<lambda>f. len_lexext" arity_sym arity_var
   by unfold_locales
 
 end
